\documentclass[12pt,letterpaper]{article}
\usepackage{fullpage}
\usepackage[top=2cm, bottom=4.5cm, left=2.5cm, right=2.5cm]{geometry}
\usepackage{amsmath,amsthm,amsfonts,amssymb,amscd}
\usepackage{lastpage}
\usepackage{fancyhdr}
\usepackage{enumerate}



% Edit these as appropriate
\newcommand\course{Machine Learning}
\newcommand\hwnumber{1}                  
\newcommand\ChiNguyen{Chi Nguyen}         
\pagestyle{fancyplain}
\headheight 35pt
\lhead{\ChiNguyen}

\chead{\textbf{\Large Homework \hwnumber}}
\rhead{\course \\ \today}
\lfoot{}
\cfoot{}
\rfoot{\small\thepage}
\headsep 1.5em

\begin{document}
    \section*{Problem 1}
        Let H denote the even that has Hansenâ€™s disease
        Let P denote the even that test positive\\
        The probability is:\\
        \begin{align*}
            P(H \mid P) &= \frac{P(PH)}{P(P)}\\
                        &= \frac{P(PH)}{P(PH) + P(PH^\complement)}\\
                        &= \frac{(0.5)(0.98)}{(0.05)(0.98) + (0.03)(0.95)}\\
                        &= 0.6323
        \end{align*}
    
    \section*{Problem 2}
        \begin{enumerate}
            \item Univariate normal distribution
                \begin{align*}
                    \int_{-\infty}^{\infty} p(x)dx 
                    &= \int_{-\infty}^{\infty}\frac{1}{{\sigma\sqrt {2\pi }}}e^{{{ - \left( {x - \mu } \right)^2 } \mathord{\left/ {\vphantom {{ - \left( {x - \mu } \right)^2 } {2\sigma ^2 }}} \right. \kern-\nulldelimiterspace} {2\sigma ^2 }}}dx \\
                    &= \int_{-\infty}^{\infty}e^{{{ - \left( {x - \mu } \right)^2 } \mathord{\left/ {\vphantom {{ - \left( {x - \mu } \right)^2 } {2\sigma ^2 }}} \right. \kern-\nulldelimiterspace} {2\sigma ^2 }}}dx \frac{1}{\sigma\sqrt {2\pi}}
                \end{align*}
                    
                
                
                \begin{equation*}
                    I = \int_{-\infty}^{\infty}e^{{{ - \left( {x - \mu } \right)^2 } \mathord{\left/ {\vphantom {{ - \left( {x - \mu } \right)^2 } {2\sigma ^2 }}} \right. \kern-\nulldelimiterspace} {2\sigma ^2 }}}dx
                      = \int_{-\infty}^{\infty}e^{-y^2/2\sigma ^2}dy
                \end{equation*}
                    
                \begin{equation*}
                    I^2 = \int_{-\infty}^{\infty}\int_{-\infty}^{\infty}e^{-x^2/2\sigma ^2}e^{-y^2/2\sigma ^2}dxdy
                        = \int_{-\infty}^{\infty}\int_{-\infty}^{\infty}e^{-(x^2+y^2)/2\sigma ^2}dxdy
                \end{equation*}
                
                With
                \begin{align*}
                    x = r\cos{\theta}\\
                    y = r\sin{\theta}
                \end{align*}
                Apply Jacobian of the change of variables, we have:
                \begin{equation*}
                    \begin{split}
                        I^2 &= \int_{0}^{2\pi}\int_{0}^{\infty}e^{-r^2/2\sigma ^2}rdrd\theta\\
                            &= 2\pi \int_{0}^{\infty}e^{-r^2/2\sigma ^2}rdr\\
                            &= 2\pi(-\sigma^2)\e^{-r^2/\sigma^2}\Big|_0^\infty\\
                            &= 2\pi\sigma^2
                    \end{split}
                \end{equation*}
                \Rightarrow I = \sqrt{2\pi\sigma^2} \Rightarrow \[\int_{-\infty}^{\infty} p(x)dx\] = 1 \Rightarrow p(x) \ normalized\\
                
                MEAN: E[X] = \(\int_{-\infty}^{\infty}xf(x)dx\) = \(\int_{-\infty}^{\infty}xe^{-(x-\mu)^2/2\sigma^2}dx\frac{1}{\sqrt{2\pi\sigma^2}}\)
        
                Let \(y = x - \mu\) \Rightarrow \(x = y + \mu\), dx = dy
                \begin{align*}
                    E(X) &= \int_{-\infty}^{\infty}(y + \mu)e^{-y^2/2\sigma^2}dy \frac{1}{\sqrt{2\pi}\sigma}\\ 
                         &= \int_{-\infty}^{\infty}ye^{-y^2/2\sigma^2}dy \frac{1}{\sqrt{2\pi}\sigma} + \int_{-\infty}^{\infty}e^{-y^2/2\sigma^2}dy \frac{\mu}{\sqrt{2\pi}\sigma}\\  &= 0 + \mu\\
                         &= \mu
                \end{align*}
                
                VAR: V[X] = \(\int_{-\infty}^{\infty}(x-\mu)^2f(x)dx\) = \(\int_{-\infty}^{\infty}y^2e^{-y^2/2\sigma^2}dy\frac{1}{\sqrt{2\pi}\sigma}\)
                \begin{align*}
                    u &= y  &  du &= dy \\
                   dv &= ye^{-y^2/2\sigma^2}dy & v &= -\sigma^2e^{-y^2/2\sigma^2}
                \end{align*}
                
                \begin{align*}
                    V[X] &= \Big[-\sigma^2ye^{-y^2/2\sigma^2}\big|_{-\infty}^\infty +\sigma^2\int_{-\infty}^{\infty}e^{-y^2/2\sigma^2}\Big]\frac{1}{\sqrt{2\pi}\sigma}\\
                         &= 0 + \sigma^2\\
                         &= \sigma^2
                \end{align*}
                
                
        \end{enumerate}
    
\end{document}
